ISA.fst
@@ -1,0 +1,210 @@
+module ISA
+
+open FStar.Math.Lib
+open FStar.Mul
+
+open Cpu
+open Memory
+open InstructionDecoder
+open Value
+
+let rec xor (a b:nat): nat =
+  match a, b with
+    | p, 0 -> p
+    | 0, p -> p
+    | _, _ -> (
+         let next_a = (arithmetic_shift_right a 1) in
+         let next_b = (arithmetic_shift_right b 1) in
+         assert(next_a < a);
+         assert(next_b < b);
+         (if (a % 2) = (b % 2) then 0 else 1) + 2*xor next_a next_b
+         )
+
+let rec xor_each_element_is_own_inverse (x:nat):
+  Lemma (ensures xor x x = 0)
+        [SMTPat (xor x x)] =
+    match x with
+      | 0 -> ()
+      | _ -> xor_each_element_is_own_inverse (arithmetic_shift_right x 1)
+
+let rec land (a b:nat): nat =
+  match a, b with
+    | p, 0 -> 0
+    | 0, p -> 0
+    | _, _ -> (
+         let next_a = (arithmetic_shift_right a 1) in
+         let next_b = (arithmetic_shift_right b 1) in
+         assert(next_a < a);
+         assert(next_b < b);
+         (if (a % 2 = 1) && (b % 2 = 1) then 1 else 0) + 2*land next_a next_b
+         )
+
+(* Instruction format:
+ *
+ *   opcode | out1 | in1 | in2 | imm
+ *  63    61 60  56 55 51 50 46 45 0
+ *)
+let parse_opcode (inst:word) = (arithmetic_shift_right inst 61) % 8
+let parse_out1 (inst:word): nat = (arithmetic_shift_right inst 56) % 32
+let parse_in1 (inst:word): nat = (arithmetic_shift_right inst 51) % 32
+let parse_in2 (inst:word): nat = (arithmetic_shift_right inst 45) % 32
+let parse_imm (inst:word): nat = inst % ((pow2 46) - 1)
+
+let sample_decoder (inst:word): decodedInstruction =
+
+  let opcode = parse_opcode inst in
+  let out1 = parse_out1 inst in
+  let in1 = parse_in1 inst in
+  let in2 = parse_in2 inst in
+  match opcode with
+  (* Store *)
+    | 0 -> { opcode; input_operands = [ Register in1; Register in2 ]; output_operands = [] }
+  (* Load *)
+    | 1 -> { opcode; input_operands = [ Register in1; Register in2 ]; output_operands = [] }
+  (* Branch *)
+    | 2 -> { opcode; input_operands = [PC; Register in1; Register in2]; output_operands = [PC] }
+  (* Arithmetic *)
+    | 3 -> { opcode; input_operands = [ Register in1; Register in2 ]; output_operands = [ Register out1 ] }
+    | 4 -> { opcode; input_operands = [ Register in1; Register in2 ]; output_operands = [ Register out1 ] }
+    | 5 -> { opcode; input_operands = [ Register in1; Register in2 ]; output_operands = [ Register out1 ] }
+    | 6 -> { opcode; input_operands = [ Register in1; Register in2 ]; output_operands = [ Register out1 ] }
+    | 7 -> { opcode; input_operands = [ Register in1; Register in2 ]; output_operands = [ Register out1 ] }
+
+let sample_decoded_instruction_length (inst:word):
+  Lemma (ensures FStar.List.length (sample_decoder inst).input_operands =
+                    (match (sample_decoder inst).opcode with
+                     | 0 -> 2
+                     | 1 -> 2
+                     | 2 -> 3
+                     | 3 -> 2
+                     | 4 -> 2
+                     | 5 -> 2
+                     | 6 -> 2
+                     | 7 -> 2
+                     )
+        )
+        [SMTPat (sample_decoder inst)]=
+  ()
+
+
+val sample_semantics: instruction_semantics sample_decoder
+let sample_semantics (di:decoder_output sample_decoder)
+                     (pre:(list (maybeBlinded #word)){
+                       (exists(s: systemState). pre = get_operands di.input_operands s) /\
+                       FStar.List.length pre = FStar.List.length di.input_operands})
+                     : instruction_result di =
+  match di.opcode with
+    (* Store *)
+    | 0 -> let address = (FStar.List.Tot.index pre 0) in
+
+    { register_writes = []; memory_ops = if Blinded? address then [] else (
+      assert(FStar.List.length di.input_operands = 2);
+      match (FStar.List.Tot.index di.input_operands 0), (FStar.List.Tot.index di.input_operands 1) with
+        | Register d, Register s -> [Store (unwrap address) s]
+        | _ -> []
+      )}
+    (* Load *)
+    | 1 -> let address = (FStar.List.Tot.index pre 0) in
+          { register_writes = [];
+            memory_ops = if Blinded? address
+                         then []
+                         else match (FStar.List.Tot.index di.input_operands 0), (FStar.List.Tot.index di.input_operands 1) with
+                               | Register d, Register s -> [Load (unwrap address) d]
+                               | _ -> []}
+    (* Branch *)
+    | 2 -> ( let pc = FStar.List.Tot.index pre 0 in
+            let a = FStar.List.Tot.index pre 1 in
+            let b = FStar.List.Tot.index pre 2 in
+            let ref: maybeBlinded #word = Clear #word 0 in
+
+            { register_writes = [if a = ref then b else pc]; memory_ops = [] } )
+    (* Add *)
+    | 3 -> ( assert(FStar.List.length pre = 2);
+            let a = FStar.List.Tot.index pre 0 in
+            let b = FStar.List.Tot.index pre 1 in
+            let result = (unwrap a) + (unwrap b) in
+            let result = if any_value_is_blinded pre then Blinded result else Clear result in
+           {
+            register_writes = [result];
+            memory_ops = [];
+          })
+    (* Sub *)
+    | 4 -> ( assert(FStar.List.length pre = 2);
+            let a = FStar.List.Tot.index pre 0 in
+            let b = FStar.List.Tot.index pre 1 in
+            let result = max 0 ((unwrap a) - (unwrap b)) in
+            let result = if any_value_is_blinded pre then Blinded result else Clear result in
+           {
+            register_writes = [result];
+            memory_ops = [];
+          })
+    (* MUL *)
+    | 5 -> ( assert(FStar.List.length pre = 2);
+            let a = FStar.List.Tot.index pre 0 in
+            let b = FStar.List.Tot.index pre 1 in
+            let result = (unwrap a) * (unwrap b) in
+            let result = if (FStar.List.Tot.index di.input_operands 0) = (FStar.List.Tot.index di.input_operands 1) then
+                            Clear 0
+                         else if any_value_is_blinded pre then
+                            Blinded result
+                         else Clear result in
+           {
+            register_writes = [result];
+            memory_ops = [];
+          })
+    (* AND *)
+    | 6 -> ( assert(FStar.List.length pre = 2);
+            let a: maybeBlinded #word = FStar.List.Tot.index pre 0 in
+            let b: maybeBlinded #word = FStar.List.Tot.index pre 1 in
+            let result: nat = land (unwrap a) (unwrap b) in
+            let result = if (a = Clear #word 0) || (b = Clear #word 0) then
+                            Clear 0
+                         else if any_value_is_blinded pre then
+                            Blinded result
+                         else Clear result in
+                         { register_writes = [result];
+                           memory_ops = [];}
+          )
+    (* XOR *)
+    | 7 -> ( assert(FStar.List.length pre = 2);
+            let a = FStar.List.Tot.index pre 0 in
+            let b = FStar.List.Tot.index pre 1 in
+            let result: nat = xor (unwrap a) (unwrap b) in
+            let result = if (FStar.List.Tot.index di.input_operands 0) = (FStar.List.Tot.index di.input_operands 1) then
+                            Clear 0
+                         else if any_value_is_blinded pre then
+                            Blinded result
+                         else Clear result in
+                         { register_writes = [result];
+                           memory_ops = [];}
+          )
+
+#set-options "--z3rlimit 10"
+let sample_semantics_are_redacting_equivalent (inst:word)
+                                      (pre:instruction_input (sample_decoder inst)):
+  Lemma (ensures (equiv_result (sample_semantics (sample_decoder inst) pre)
+                               (sample_semantics (sample_decoder inst)
+                                                 (redacted_instruction_inputs_are_instruction_inputs (sample_decoder inst) pre)))) =
+  ()
+
+let add_instruction_works_correctly (inst:word)
+                                    (pre:(list (maybeBlinded #word)){
+                                      (exists(s: systemState). pre = get_operands (sample_decoder inst).input_operands s) /\
+                                      FStar.List.length pre = FStar.List.length (sample_decoder inst).input_operands}):
+    Lemma (requires parse_opcode inst = 3)
+          (ensures  unwrap (FStar.List.Tot.hd (sample_semantics (sample_decoder inst) pre).register_writes) = (unwrap (FStar.List.Tot.index pre 0)) + (unwrap (FStar.List.Tot.index pre 1)) ) =
+    ()
+
+
+let xor_instruction_works_correctly (inst:word)
+                                    (pre:(list (maybeBlinded #word)){
+                                      (exists(s: systemState). pre = get_operands (sample_decoder inst).input_operands s) /\
+                                      FStar.List.length pre = FStar.List.length (sample_decoder inst).input_operands}):
+    Lemma (requires parse_opcode inst = 7)
+          (ensures  unwrap (FStar.List.Tot.hd (sample_semantics (sample_decoder inst) pre).register_writes)
+                    = xor (unwrap (FStar.List.Tot.index pre 0)) (unwrap (FStar.List.Tot.index pre 1)) ) =
+    let di = sample_decoder inst in
+    if (FStar.List.Tot.index di.input_operands 0) = (FStar.List.Tot.index di.input_operands 1) then
+      assert(xor (unwrap (FStar.List.Tot.index pre 0)) (unwrap (FStar.List.Tot.index pre 1)) = 0)
+    else
+      ()
